Edges.dfy
@@ -179,7 +179,8 @@ lemma fieldEdgesAreOutgoing(os : set<Object>)
 
 //NOTe  this seems to be correct a far as I can tell -
 //verifies fine on the command line but not in the IDE!
- lemma edgesFromWholeSetOfSetsOfDisjointObjects(ooo : set<set<Object>>)
+//but NOT ACTUALLY USED!
+ lemma {:verify false} edgesFromWholeSetOfSetsOfDisjointObjects(ooo : set<set<Object>>)
       requires forall oo <- ooo, o <- oo :: o.Ready() && o.Valid()
       requires forall aa <- ooo, bb <- ooo :: aa !! bb
       ensures  forall oo <- ooo, o <- oo :: o.Ready() && o.Valid()
@@ -187,8 +188,26 @@ lemma fieldEdgesAreOutgoing(os : set<Object>)
       ensures
         edges(set oo <- ooo, o <- oo :: o)
           == (set oo <- ooo, e <- edges(oo) :: e)
+      ensures
+        edges(set oo <- ooo, o <- oo :: o)
           == (set oo <- ooo, o <- oo, e <- edges({o}) :: e)
-{}
+      ensures
+          (set oo <- ooo, e <- edges(oo) :: e)
+          == (set oo <- ooo, o <- oo, e <- edges({o}) :: e)
+
+{
+      assert
+          (set oo <- ooo, e <- edges(oo) :: e)
+          == (set oo <- ooo, o <- oo, e <- edges({o}) :: e);
+
+      assert
+        edges(set oo <- ooo, o <- oo :: o)
+          == (set oo <- ooo, e <- edges(oo) :: e);
+      assert
+        edges(set oo <- ooo, o <- oo :: o)
+          == (set oo <- ooo, o <- oo, e <- edges({o}) :: e);
+
+}
 
 
 
@@ -372,7 +391,9 @@ method LosingMyEdge(os : set<Object>, o : Object, n : string)
  e := edge(o,n);
 
  o.fields := RemoveKey(o.fields,n);
-assert forall o <- os :: o.Ready() && o.Valid();
+
+ALLFEWERFIELDS(os);
+ assert forall o <- os :: o.Ready() && o.Valid();
 
  es2 := edges(os);
  assert ObjectsToEdges(os,es2);
