ScratchMonkey.dfy
@@ -31,6 +31,9 @@ lemma AMFUCKED(a : Object)
 
 lemma InTheBox(a : Object, m : Klon)
   requires  COK(a, m.oHeap)
+  requires a.Ready()
+  requires a.AllOutgoingReferencesWithinThisHeap(m.m.Keys+{a})
+
   requires  a.allExternalOwners() <= m.m.Keys
   requires  a.allExternalBounds() <= m.m.Keys
   ensures   COK(a, m.m.Keys+{a})
@@ -38,28 +41,40 @@ lemma InTheBox(a : Object, m : Klon)
   reveal COK();
 assert COK(a, m.oHeap);
 assert a.Ready();
-assert a.OvenReady();
 
 assert a.AMFX <= m.m.Keys;
 assert a.AMFB <= m.m.Keys;
 assert a.AMFO == a.AMFX+{a};
 assert a.AMFO <= m.m.Keys+{a};
-// var context := m.m.Keys+{a};
-// assert
-//     && (a in context)
-//     //&& (a.AMFO <= context)
-//     //&& (a.AMFB <= context) //sgould be derivable, AMFB <= AMFO
-//     && (a.AMFB <= a.AMFO <= context)
-//     && (forall oo <- a.AMFO :: oo.Ready())
-//     && (forall o <- (a.AMFO - {a}), ooo <- o.AMFO :: a.AMFO >= o.AMFO > ooo.AMFO)
-//   //  && (a.TRUMP()||(a.Ready() && a.Valid()))
-//     && (a.Ready())
-//     && (a.Valid())
-//     && (a.AllOutgoingReferencesAreOwnership(context))
-// //    && (a.AllOutgoingReferencesWithinThisHeap(context))
-//     && (a.AllOwnersAreWithinThisHeap(context))
-//
-//     && AllTheseOwnersAreFlatOK(a.AMFO - {a})
-//     ;
+
+assert a.AllOutgoingReferencesAreOwnership({});
+
+var context := m.m.Keys+{a};
+
+assert a.AllOutgoingReferencesAreOwnership({});
+
+
+
+assert
+    && (a in context)
+    //&& (a.AMFO <= context)
+    //&& (a.AMFB <= context) //sgould be derivable, AMFB <= AMFO
+    && (a.AMFB <= a.AMFO <= context)
+    && (forall oo <- a.AMFO :: oo.Ready())
+    && (forall o <- (a.AMFO - {a}), ooo <- o.AMFO :: a.AMFO >= o.AMFO > ooo.AMFO)
+  //  && (a.TRUMP()||(a.Ready() && a.Valid()))
+    && (a.Ready())
+    && (a.Valid())
+    && (a.AllOutgoingReferencesAreOwnership(context))
+    && (a.AllOutgoingReferencesWithinThisHeap(context))
+    && (a.AllOwnersAreWithinThisHeap(context))
+
+    && AllTheseOwnersAreFlatOK(a.AMFO - {a})
+    ;
+
+
+  reveal COK();
+  assert COK(a, context);
+  assert COK(a, m.m.Keys+{a});
 
 }
